added omega semantics

IMP--_To_SAS+/Correctness.thy
@@ -3,110 +3,261 @@
 section "Correctness"
 
 theory Correctness imports Reduction
-begin
+begin 
 
-definition imp_minus_sas_plus_equivalent_states :: "com \<Rightarrow> com \<Rightarrow> nat \<Rightarrow> imp_state \<Rightarrow> sas_state \<Rightarrow> bool" where
-"imp_minus_sas_plus_equivalent_states c c1 r is ss = (ss PC = Some (Num (index_of (all_subprograms c) c1)) 
-  \<and> list_all (\<lambda>v. ss (VN v) = Some (Num (is v)) \<or> (is v > r \<and> ss (VN v) = Some \<omega>)) (enumerate_variables c))"  
+definition imp_minus_sas_plus_equivalent_states :: "com \<Rightarrow> com \<Rightarrow> imp_state \<Rightarrow> sas_state \<Rightarrow> bool" where
+"imp_minus_sas_plus_equivalent_states c c1 is ss = (ss PC = Some (PCV c1) 
+  \<and> list_all (\<lambda>v. ss (VN v) = Some (EV (is v))) (enumerate_variables c))"
 
-lemma imp_minus_sas_plus_equivalent_states_assign:
-  assumes "t' \<le> t"
-    "imp_minus_sas_plus_equivalent_states c (x ::= a) (t' * max_constant c) s ss1"
-  shows "imp_minus_sas_plus_equivalent_states c SKIP ((t' - Suc 0) * max_constant c)
-     (\<lambda>y. if y = x then aval a s else s y)
-     (ss1(VN x \<mapsto> Num (aval a s), PC \<mapsto> Num (index_of (all_subprograms c) SKIP)))"
+lemma [simp]: "imp_minus_sas_plus_equivalent_states c c1 is ss \<Longrightarrow> v \<in> set (enumerate_variables c)
+  \<Longrightarrow> is v = Num 0 \<longleftrightarrow> ss (VN v) = Some (EV (Num 0))"
+  by (auto simp: imp_minus_sas_plus_equivalent_states_def list_all_def)
+
+lemma [simp]: "[VN v \<mapsto> y, PC \<mapsto> x] \<subseteq>\<^sub>m s = (s PC = Some x \<and> s (VN v) = Some y)"
+  by (auto simp: map_le_def)
+
+lemma [simp]: "[PC \<mapsto> x] \<subseteq>\<^sub>m s \<longleftrightarrow> (s PC = Some x)" 
+  by (auto simp: map_le_def)
+
+lemma greater_helper: "(x :: nat) > 0 \<Longrightarrow> b \<le> c \<Longrightarrow> x * c < d \<Longrightarrow> (x - 1) * c < d - b"   
+  by (simp add: mult_eq_if)
+
+lemma map_of_list_update: "distinct (map fst l) \<Longrightarrow> length l > 0 \<Longrightarrow> fst (l ! 0) = x  \<Longrightarrow> z \<noteq> x
+  \<Longrightarrow> map_of (list_update l 0 (x, y)) z = map_of l z"
+  by (induction l) auto
+
+lemma [simp]: assumes "op \<in> set (com_to_operators c d)"
+  shows "map_of (list_update (effect_of op) 0 (PC, y)) = (map_of (effect_of op))(PC \<mapsto> y)"
 proof -
-  let ?ss2 = "ss1(VN x \<mapsto> Num (t * max_constant c), PC \<mapsto> Num (index_of (all_subprograms c) SKIP))"
-  let ?is2 = "\<lambda>a. if a = x then aval (A (N (t * max_constant c))) s else s a"
-  let ?r1 = "t' * max_constant c"
-  let ?r2 = "(t' - Suc 0) * max_constant c"
-  have "v \<in> set (enumerate_variables c)
-     \<Longrightarrow> ?ss2 (VN v) = Some (Num (?is2 v)) \<or> (?is2 v > ?r2 \<and> ?ss2 (VN v) = Some \<omega>)" for v 
-  proof -
-    assume "v \<in> set (enumerate_variables c)"
-    moreover have "list_all (\<lambda>v. ss1 (VN v) 
-      = Some (Num (s v)) \<or> (s v > ?r1 \<and> ss1 (VN v) = Some \<omega>)) (enumerate_variables c)"
-      using assms by(auto simp: imp_minus_sas_plus_equivalent_states_def)
-    ultimately have "ss1 (VN v) = Some (Num (s v)) \<or> (s v > ?r1 \<and> ss1 (VN v) = Some \<omega>)" 
-      by (simp add: list_all_iff)
-    then show ?thesis using diff_mult_distrib by auto
-  qed
-  then show ?thesis using assms 
-    by (fastforce simp: imp_minus_sas_plus_equivalent_states_def list_all_iff)
+  have "map_of (list_update (effect_of op) 0 (PC, y)) x = ((map_of (effect_of op))(PC \<mapsto> y)) x" for x
+    using assms com_to_operators_variables_distinct effect_nonempty 
+      map_of_list_update[where ?l = "effect_of op"]
+    by (auto) 
+      (metis effect_nonempty fst_of_effect map_of_eq_Some_iff set_update_memI update_preserve_distinct)
+  then show ?thesis by auto
 qed
 
-lemma "a \<noteq> c \<Longrightarrow> f(a \<mapsto> b, c \<mapsto> d) = (\<lambda>x. if x = a then Some b else (f(c \<mapsto> d)) x)" 
-  by auto
+lemma [simp]: assumes "op \<in> set (com_to_operators c d)"
+  shows "map_of (list_update (precondition_of op) 0 (PC, y)) = (map_of (precondition_of op))(PC \<mapsto> y)"
+proof -
+  have "map_of (list_update (precondition_of op) 0 (PC, y)) x = ((map_of (precondition_of op))(PC \<mapsto> y)) x" for x
+    using assms com_to_operators_variables_distinct precondition_nonempty 
+      map_of_list_update[where ?l = "precondition_of op"]
+    by (auto) 
+     (metis precondition_nonempty fst_of_precondition map_of_eq_Some_iff set_update_memI update_preserve_distinct)
+  then show ?thesis by auto
+qed
 
+lemma pc_of_op: "op \<in> set (com_to_operators c2 d) 
+  \<Longrightarrow> imp_minus_sas_plus_equivalent_states c c1 is ss2 \<Longrightarrow> ss1 \<then>\<^sub>+ op = ss2
+  \<Longrightarrow> pc_to_com (effect_of op) = c1" 
+  by (auto simp: imp_minus_sas_plus_equivalent_states_def com_to_operators_variables_distinct)
 
-lemma imp_minus_minus_to_sas_plus_single_step:
-   "(c1, is1) \<rightarrow> (c2, is2) \<Longrightarrow> cs = all_subprograms c \<Longrightarrow> c1 \<in> set cs \<Longrightarrow> t' \<le> t \<Longrightarrow> t > 0
-  \<Longrightarrow> imp_minus_sas_plus_equivalent_states c c1 (t' *  (max_constant c)) is1 ss1 
-  \<Longrightarrow> (\<exists>op \<in> set (com_to_operators cs c1 (domain c t)). \<exists>ss2.
-     imp_minus_sas_plus_equivalent_states c c2 ((t' - 1) *  (max_constant c)) is2 ss2
-    \<and> is_operator_applicable_in ss1 op
-    \<and> execute_operator_sas_plus ss1 op = ss2)"
-proof (induction c1 is1 c2 is2 rule: small_step_induct)
-  case (Assign x a s)
-  let ?i = "index_of cs (x ::= a)"
-  let ?j = "index_of cs SKIP"
-  have "SKIP \<in> set (all_subprograms c)" using SKIP_in_enumerate_subprograms by simp
-  moreover then have "SKIP \<in> set cs" using Assign by blast
-  have "aval a s \<le> t * (max_constant c) \<or> aval a s > t * (max_constant c)" by auto
-  show ?case
+lemma effect_in_updated[simp]: 
+  assumes "op' \<in> set (com_to_operators c d)" 
+    "map_of (precondition_of op') = (map_of (precondition_of op))(PC \<mapsto> PCV c)"
+    "map_of (effect_of op') = (map_of (effect_of op))(PC \<mapsto> PCV (pc_to_com (effect_of op')))"
+    "s \<then>\<^sub>+ op = s'"
+  shows "s(PC \<mapsto> PCV c) \<then>\<^sub>+ op' = s'(PC \<mapsto> PCV (pc_to_com (effect_of op')))" 
+proof -
+  have "(s(PC \<mapsto> PCV c)  \<then>\<^sub>+ op') x = (s'(PC \<mapsto> PCV (pc_to_com (effect_of op')))) x" for x
+    using assms PC_in_effect_precondition com_to_operators_variables_distinct apply auto
+    by (metis fun_upd_other map_add_def)
+  then show ?thesis by auto
+qed
+
+lemma applicable_in_PC_updated: "m \<subseteq>\<^sub>m s(PC \<mapsto> y) \<Longrightarrow> s PC = Some x \<Longrightarrow> m(PC \<mapsto> x) \<subseteq>\<^sub>m s"
+  by (simp add: map_le_def)
+
+lemma [simp]: "(s(PC \<mapsto> y) ++ (map_of m))(PC \<mapsto> x) = (s ++ (map_of m))(PC \<mapsto> x)"
+proof -
+  have "((s(PC \<mapsto> y) ++ (map_of m))(PC \<mapsto> x)) z = ((s ++ (map_of m))(PC \<mapsto> x)) z" for z
+    by (simp add: fun_upd_def map_add_def)
+  then show ?thesis by auto
+qed
+
+lemma sas_plus_to_imp_minus_minus_single_step:
+  "op \<in> set (com_to_operators c1 (domain c t)) \<Longrightarrow> cs = enumerate_subprograms c 
+  \<Longrightarrow> c1 \<in> set (enumerate_subprograms c) \<Longrightarrow> t > 0 
+  \<Longrightarrow> imp_minus_sas_plus_equivalent_states c c1 is1 ss1
+  \<Longrightarrow> is_operator_applicable_in ss1 op
+  \<Longrightarrow> ss1 \<then>\<^sub>+ op = ss2
+  \<Longrightarrow> the (ss2 PC) = PCV c2
+  \<Longrightarrow> (\<exists>is2. ((c1, is1) \<rightarrow>\<^bsub>t * max_constant c\<^esub> (c2, is2)) \<and>
+      imp_minus_sas_plus_equivalent_states c c2 is2 ss2)"
+proof (induction c1 arbitrary: op ss1 ss2 is1 c2)
+  case (Assign x a)
+  let ?is2 = "is1(x := eval a is1 (t * max_constant c))"
+  have "imp_minus_sas_plus_equivalent_states c SKIP ?is2 ss2" using Assign
   proof (cases a)
     case (A atom)
     then show ?thesis
     proof (cases atom)
       case (N val)
-      let ?op = "\<lparr> precondition_of = [(PC, Num ?i)], 
-                  effect_of = [(PC, Num ?j), (VN x, (if val \<le> t * (max_constant c) then Num val else \<omega>))]\<rparr>"
-      let ?ss2 = "ss1(VN x \<mapsto> Num val, PC \<mapsto> Num ?j)"
-      have *: "val \<le> max_constant c" using enumerate_subprograms_max_constant Assign A N by fastforce
-      then have "Num val \<in> set (domain c t)" using Assign by (auto simp: domain_def Let_def) 
-          (metis Suc_lessI add.right_neutral atLeastLessThan_iff image_eqI lambda_zero le_0_eq le_less_trans le_neq_implies_less n_less_m_mult_n nat_le_linear times_nat.simps(2))
-      moreover have "?op \<in> set (com_to_operators cs (x ::= a) (domain c t))" 
-        using A N by (auto simp: domain_def Let_def)
-      moreover have "is_operator_applicable_in ss1 ?op" using Assign 
-        by (auto simp: imp_minus_sas_plus_equivalent_states_def)
-           (metis (no_types) fun_upd_triv map_le_empty map_le_upd)
-      moreover have "execute_operator_sas_plus ss1 ?op = ?ss2" using Assign A N * 
-        by auto (metis gr0_implies_Suc times_nat.simps trans_le_add1)
-      moreover have "imp_minus_sas_plus_equivalent_states c SKIP ((t' - Suc 0) * max_constant c) 
-        (\<lambda>y. if y = x then val else s y)
-        ?ss2" using Assign A N 
-        by (smt atomVal.simps aval.simps imp_minus_sas_plus_equivalent_states_def list_all_iff imp_minus_sas_plus_equivalent_states_assign[OF Assign(3) Assign(5)])
-      ultimately show ?thesis using Assign A N by fastforce
+      then show ?thesis using Assign A
+        by (auto simp: imp_minus_sas_plus_equivalent_states_def list_all_def)
     next
       case (V var)
-      then show ?thesis sorry
+      have "var \<in> set (enumerate_variables c)" 
+        using Assign A V enumerate_subprograms_enumerate_variables by fastforce
+      then show ?thesis using Assign A V 
+        by (auto simp: imp_minus_sas_plus_equivalent_states_def list_all_def)
     qed
+  qed (auto simp: enumerate_variables_def imp_minus_sas_plus_equivalent_states_def list_all_def 
+        split: EVal.splits)
+  then show ?case using Assign imp_minus_sas_plus_equivalent_states_def by auto
+next
+  case (Seq cA cB)
+  have "cA = SKIP \<or> cA \<noteq> SKIP" by auto
+  then show ?case
+  proof (elim disjE)
+    assume "cA = SKIP"
+    then show ?thesis using Seq by (fastforce simp: imp_minus_sas_plus_equivalent_states_def)
   next
-    case (Plus x21 x22)
-    then show ?thesis sorry
-  next
-    case (Sub x31 x32)
-    then show ?thesis sorry
+    assume "cA \<noteq> SKIP"
+    then obtain op' where op'_def: "op' \<in> set (com_to_operators cA (domain c t)) 
+      \<and> op = (let c1' = pc_to_com (effect_of op') in 
+      \<lparr> precondition_of = 
+        list_update (precondition_of op') 0 (PC, PCV (cA ;; cB)),
+        effect_of = 
+        list_update (effect_of op') 0 (PC, PCV (c1' ;; cB))\<rparr>)" using Seq by auto
+    let ?c1' = "pc_to_com (effect_of op')"
+    let ?ss1' = "ss1(PC \<mapsto> PCV cA)"
+    let ?ss2' = "ss2(PC \<mapsto> PCV ?c1')"
+    have "cA \<in> set (enumerate_subprograms (cA ;; cB))" using c_in_all_subprograms_c by auto
+    then have "cA \<in> set (enumerate_subprograms c)" 
+      using Seq enumerate_subprograms_transitive by blast
+    moreover have "imp_minus_sas_plus_equivalent_states c cA is1 ?ss1'" 
+      using Seq by (auto simp: imp_minus_sas_plus_equivalent_states_def)
+    moreover have "map_of (precondition_of op') = (map_of (precondition_of op))(PC \<mapsto> PCV cA)"
+      using op'_def Seq com_to_operators_variables_distinct by auto
+    moreover then have "is_operator_applicable_in ?ss1' op'" 
+      using Seq op'_def by auto
+    moreover have "map_of (effect_of op') = map_of (effect_of op)(PC \<mapsto> PCV (pc_to_com (effect_of op')))"
+       using op'_def Seq com_to_operators_variables_distinct by auto
+    moreover then have "?ss1' \<then>\<^sub>+ op' = ?ss2'" using Seq op'_def by auto
+    ultimately have "\<exists>is2. (cA, is1) \<rightarrow>\<^bsub>t * max_constant c\<^esub> (?c1', is2) \<and>
+      imp_minus_sas_plus_equivalent_states c ?c1' is2 ?ss2'" using Seq op'_def by fastforce
+    then show ?thesis using Seq op'_def 
+      by (fastforce simp: imp_minus_sas_plus_equivalent_states_def)
   qed
 next
-  case (Seq1 c\<^sub>2 s)
-  then show ?case sorry
+  case (If b cA cB)
+  then have "c2 = (if ss1 (VN b) \<noteq> Some (EV (Num 0)) then cA else cB)" by auto
+  moreover have "b \<in> set (enumerate_variables (IF b\<noteq>0 THEN cA ELSE cB))" by auto
+  moreover then have "b \<in> set (enumerate_variables c)" 
+    using If enumerate_subprograms_enumerate_variables by blast
+  ultimately show ?case using If enumerate_subprograms_enumerate_variables 
+    by (fastforce simp: imp_minus_sas_plus_equivalent_states_def)
 next
-  case (Seq2 c\<^sub>1 s c\<^sub>1' s' c\<^sub>2)
-  then show ?case sorry
+  case (While b cA)
+  then have "c2 = (if ss1 (VN b) \<noteq> Some (EV (Num 0)) then cA ;; WHILE b \<noteq>0 DO cA else SKIP)" 
+    by auto
+  moreover have "b \<in> set (enumerate_variables (WHILE b\<noteq>0 DO cA))" by auto
+  moreover then have "b \<in> set (enumerate_variables c)" 
+    using While enumerate_subprograms_enumerate_variables by blast
+  ultimately show ?case using While enumerate_subprograms_enumerate_variables 
+    by (fastforce simp: imp_minus_sas_plus_equivalent_states_def)
+qed auto
+
+lemma imp_minus_minus_to_sas_plus_single_step:
+   "(c1, is1) \<rightarrow>\<^bsub>r\<^esub> (c2, is2) \<Longrightarrow> cs = enumerate_subprograms c \<Longrightarrow> r = t * max_constant c 
+  \<Longrightarrow> c1 \<in> set cs \<Longrightarrow> t > 0 
+  \<Longrightarrow> (\<forall>v. EV (is1 v) \<in> set (domain c t))
+  \<Longrightarrow> imp_minus_sas_plus_equivalent_states c c1 is1 ss1
+  \<Longrightarrow> (\<exists>op \<in> set (com_to_operators c1 (domain c t)). \<exists>ss2.
+     imp_minus_sas_plus_equivalent_states c c2 is2 ss2
+    \<and> is_operator_applicable_in ss1 op
+    \<and> execute_operator_sas_plus ss1 op = ss2)"
+proof (induction c1 is1 r c2 is2 arbitrary: ss1 rule: \<omega>_small_step_induct)
+  case (Assign x a s r)
+  let ?ss2 = "ss1(VN x \<mapsto> EV (eval a s (t * max_constant c)), PC \<mapsto> PCV SKIP)"
+  have "(\<exists>op \<in> set (com_to_operators (x ::= a) (domain c t)). 
+     imp_minus_sas_plus_equivalent_states c SKIP (s(x := eval a s (t * max_constant c)))  ?ss2
+    \<and> is_operator_applicable_in ss1 op
+    \<and> execute_operator_sas_plus ss1 op = ?ss2)" using Assign
+  proof (cases a)
+    case (A atom)
+    then show ?thesis
+    proof (cases atom)
+      case (N val)
+      then show ?thesis using Assign A
+        by (auto simp: imp_minus_sas_plus_equivalent_states_def list_all_def)
+    next
+      case (V var)
+      have "var \<in> set (enumerate_variables c)" 
+        using Assign A V enumerate_subprograms_enumerate_variables by fastforce
+      then show ?thesis using Assign A V
+        by (auto simp: imp_minus_sas_plus_equivalent_states_def list_all_def)
+    qed
+  next
+    case (Plus var val)
+    then show ?thesis using Assign Plus 
+        enumerate_subprograms_enumerate_variables enumerate_variables_def
+      by (auto simp: imp_minus_sas_plus_equivalent_states_def list_all_def split: EVal.splits)
+  next
+    case (Sub var val)
+    then show ?thesis using Assign Sub 
+        enumerate_subprograms_enumerate_variables enumerate_variables_def
+      by (auto simp: imp_minus_sas_plus_equivalent_states_def list_all_def split: EVal.splits)
+  qed 
+  then show ?case using Assign by blast
+next
+  case (Seq2 c\<^sub>1 s r c\<^sub>1' s' c\<^sub>2)
+  let ?ss1' = "ss1(PC \<mapsto> PCV c\<^sub>1)"
+  have "c\<^sub>1 \<in> set (enumerate_subprograms (c\<^sub>1 ;; c\<^sub>2))" using c_in_all_subprograms_c by auto
+  then have "c\<^sub>1 \<in> set (enumerate_subprograms c)" using Seq2 enumerate_subprograms_transitive by blast
+  then have "(\<exists>op' \<in> set (com_to_operators c\<^sub>1 (domain c t)). \<exists>ss2'.
+   imp_minus_sas_plus_equivalent_states c c\<^sub>1' s' ss2'
+    \<and> is_operator_applicable_in ?ss1' op'
+    \<and> execute_operator_sas_plus ?ss1' op' = ss2')" 
+    using Seq2 by (auto simp: imp_minus_sas_plus_equivalent_states_def)
+  then obtain op' ss2' where op'_def: "(op' \<in> set (com_to_operators c\<^sub>1 (domain c t)) \<and>
+   imp_minus_sas_plus_equivalent_states c c\<^sub>1' s' ss2'
+    \<and> is_operator_applicable_in ?ss1' op'
+    \<and> execute_operator_sas_plus ?ss1' op' = ss2')" by blast
+  let ?op = "\<lparr> precondition_of = 
+        list_update (precondition_of op') 0 (PC, PCV (c\<^sub>1 ;; c\<^sub>2)),
+        effect_of = 
+        list_update (effect_of op') 0 (PC, PCV (c\<^sub>1' ;; c\<^sub>2))\<rparr>"
+  let ?ss2 = "ss2'(PC \<mapsto> PCV (c\<^sub>1' ;; c\<^sub>2))"
+  have "?op \<in> set (com_to_operators (c\<^sub>1 ;; c\<^sub>2) (domain c t))" 
+    using Seq2 op'_def by (auto simp: pc_of_op)
+  moreover have "imp_minus_sas_plus_equivalent_states c (c\<^sub>1' ;; c\<^sub>2) s' ?ss2" 
+    using op'_def by (auto simp: imp_minus_sas_plus_equivalent_states_def)
+  moreover have "is_operator_applicable_in ss1 ?op" 
+    using op'_def Seq2 by (auto simp: applicable_in_PC_updated imp_minus_sas_plus_equivalent_states_def)
+  moreover have "execute_operator_sas_plus ss1 ?op = ?ss2"
+    using Seq2 op'_def by (auto simp: imp_minus_sas_plus_equivalent_states_def)
+  ultimately show ?case using Seq2 by blast
 next
   case (IfTrue s b c\<^sub>1 c\<^sub>2)
-  then show ?case sorry
+  then have "b \<in> set (enumerate_variables c)" 
+    using enumerate_subprograms_enumerate_variables by fastforce
+  then show ?case using IfTrue 
+    by (auto simp: imp_minus_sas_plus_equivalent_states_def)
+     (metis (mono_tags, lifting) list_all_iff)
 next
   case (IfFalse s b c\<^sub>1 c\<^sub>2)
-  then show ?case sorry
+  then have "b \<in> set (enumerate_variables c)" 
+    using enumerate_subprograms_enumerate_variables by fastforce
+  then show ?case using IfFalse
+    by (auto simp: imp_minus_sas_plus_equivalent_states_def)
 next
-  case (WhileTrue s b c)
-  then show ?case sorry
+  case (WhileTrue s b c1)
+  then have "b \<in> set (enumerate_variables c)" 
+    using enumerate_subprograms_enumerate_variables by fastforce
+  then show ?case using WhileTrue 
+    by (auto simp: imp_minus_sas_plus_equivalent_states_def)
+      (metis (mono_tags, lifting) list_all_iff)
 next
-  case (WhileFalse s b c)
-  then show ?case sorry
-qed
+  case (WhileFalse s b c1)
+  then have "b \<in> set (enumerate_variables c)" 
+    using enumerate_subprograms_enumerate_variables by fastforce
+  then show ?case using WhileFalse
+    by (auto simp: imp_minus_sas_plus_equivalent_states_def)
+qed (auto simp: imp_minus_sas_plus_equivalent_states_def)
+  
       
 
 end
