IMP--_To_SAS+/Domains.thy
@@ -95,15 +95,4 @@ proof (induction t arbitrary: c2 s2 v1)
   qed
 qed auto
 
-datatype domain_element = Num val | \<omega> 
-
-definition domain :: "com \<Rightarrow> nat \<Rightarrow> domain_element list" where
-"domain c t = (let m = max_constant c in map Num [0 ..<(t * m + 1)]) @ [\<omega>]"
-
-lemma zero_in_domain[simp]: "ListMem (Num 0) (domain c t)"
-  by (auto simp: domain_def Let_def ListMem_iff)
-
-lemma omega_in_domain[simp]: "ListMem \<omega> (domain c t)"
-  by (auto simp: domain_def Let_def ListMem_iff)
-
 end
