IMP--_To_SAS+/Reduction.thy
@@ -2,434 +2,186 @@
 
 section "Reduction"
 
-theory Reduction imports Domains "Verified_SAT_Based_AI_Planning.SAS_Plus_Representation"
+theory Reduction imports  "Verified_SAT_Based_AI_Planning.SAS_Plus_Representation" Omega_Small_StepT
 begin
+
+datatype domain_element = EV EVal | PCV com
+
+definition domain :: "com \<Rightarrow> nat \<Rightarrow> domain_element list" where
+"domain c t = (let m = max_constant c in map (\<lambda>i. EV (Num i))  [0 ..<(t * m + 1)]) @ [EV \<omega>]"
+
+lemma zero_in_domain[simp]: "ListMem (EV (Num 0)) (domain c t)"
+  by (auto simp: domain_def Let_def ListMem_iff)
+
+lemma omega_in_domain[simp]: "ListMem (EV \<omega>) (domain c t)"
+  by (auto simp: domain_def Let_def ListMem_iff)
+
+lemma [simp]: "(EV \<omega>) \<in> set (domain c t)"
+  by (auto simp: domain_def Let_def ListMem_iff)
+
+lemma num_in_domain_iff[simp]: "(EV (Num x)) \<in> set (domain c t) = (x \<le> t * (max_constant c))"
+  by (auto simp: domain_def Let_def)
+
+lemma [simp]: "((PCV i) \<in> set (domain c t)) = False" 
+  by (auto simp: domain_def Let_def)
 
 datatype variable = VN vname | PC
 
 type_synonym operator = "(variable, domain_element) sas_plus_operator"
-type_synonym sas_state = "(variable, domain_element) state"
-type_synonym imp_state = AExp.state
+type_synonym sas_state = "(variable, domain_element) State_Variable_Representation.state"
+type_synonym imp_state = EState
 type_synonym problem = "(variable, domain_element) sas_plus_problem"
 
-fun all_subprograms :: "com \<Rightarrow> com list" where
-"all_subprograms (SKIP) = [SKIP]" |
-"all_subprograms (Assign v aexp) = [(Assign v aexp), SKIP]" |
-"all_subprograms (c1 ;; c2) = (map (\<lambda> c. c ;; c2) (all_subprograms c1)) @ all_subprograms c1 
-  @ all_subprograms c2" |
-"all_subprograms (If v c1 c2) = [(If v c1 c2)] @ all_subprograms c1 @ all_subprograms c2" |
-"all_subprograms (While v c) = [(While v c), SKIP] @ all_subprograms c @ 
-  (map (\<lambda> x. x ;; (While v c)) (all_subprograms c))"
+definition pc_to_com :: "(variable \<times> domain_element) list \<Rightarrow> com" where
+"pc_to_com l = (case  l ! 0 of (_, PCV x) \<Rightarrow> x)"
 
-definition enumerate_subprograms :: "com \<Rightarrow> com list" where
-"enumerate_subprograms c = remdups (all_subprograms c)"
-
-fun all_variables :: "com \<Rightarrow> vname list" where
-"all_variables (SKIP) = []" |
-"all_variables (Assign v aexp) = [ v ] @ (case aexp of 
-  A a \<Rightarrow> (case a of V v2 \<Rightarrow> [ v2 ] | N _ \<Rightarrow> []) |
-  Plus a b \<Rightarrow> [ a ] |
-  Sub a b \<Rightarrow> [ a ])" |
-"all_variables (c1 ;; c2) = []" |
-"all_variables (If v c1 c2) = [ v ]" |
-"all_variables (While v c) = [ v ]"
-
-definition enumerate_variables :: "com \<Rightarrow> vname list" where
-"enumerate_variables c = remdups (concat (map all_variables (enumerate_subprograms c)))"
-
-declare enumerate_subprograms_def[simp] 
-
-lemma c_in_all_subprograms_c: "c \<in> set (enumerate_subprograms c)" 
-  by (induction c) auto
-
-lemma enumerate_subprograms_complete_step: "(c1, s1) \<rightarrow> (c2, s2) 
-  \<Longrightarrow> c2 \<in> set (enumerate_subprograms c1)"
-apply (induction c1 s1 c2 s2 rule: small_step_induct)
-  using c_in_all_subprograms_c apply(auto)
-done
-
-lemma enumerate_subprograms_transitive: "c2 \<in> set (enumerate_subprograms c1) \<Longrightarrow> 
-  c3 \<in> set (enumerate_subprograms c2) \<Longrightarrow> c3 \<in> set (enumerate_subprograms c1)"
-proof (induction c1 arbitrary: c2 c3 rule: all_subprograms.induct)
-  case (4 v c4 c5)
-  then have "(c2 = (If v c4 c5)) \<or> (c2 \<in> set (all_subprograms c4)) 
-              \<or> (c2 \<in> set (all_subprograms c5))"
-      by (metis Un_iff all_subprograms.simps append.simps append.simps enumerate_subprograms_def set_ConsD set_append set_remdups)
-  then show ?case
-  proof (elim disjE)
-    assume "c2 \<in> set (all_subprograms c5)" 
-    then show ?thesis using 4 by auto
-  next
-    assume "c2 \<in> set (all_subprograms c4)"
-    then show ?thesis using 4 by auto
-  next
-    assume "c2 = (If v c4 c5)"
-    then show ?thesis using 4 by auto
-  qed
-next
-  case (5 v c)
-  then have "c2 \<in> set (all_subprograms (While v c))" by (metis enumerate_subprograms_def set_remdups)
-  then have "c2 \<in> set ([While v c, SKIP] @ all_subprograms c @ map (\<lambda> x. x ;; (While v c)) (all_subprograms c))" 
-    by (metis all_subprograms.simps enumerate_subprograms_def map_eq_conv set_append set_remdups) 
-  then have "(c2 = (While v c)) \<or> c2 = SKIP \<or> (c2 \<in> set (all_subprograms c)) 
-              \<or> (c2 \<in> set (map (\<lambda> x. x ;; (While v c)) (all_subprograms c)))" by simp
-  then show ?case
-  proof (elim disjE)
-    assume "c2 = (While v c)"
-    then show ?thesis using 5 by auto
-  next
-    assume "c2 = SKIP"
-    then show ?thesis using 5 by auto
-  next
-    assume "c2 \<in> set (all_subprograms c)"
-    then show ?thesis using 5 
-      by (metis Un_iff all_subprograms.simps enumerate_subprograms_def set_append set_remdups)
-  next
-    assume "c2 \<in> set (map (\<lambda> x. x ;; (While v c)) (all_subprograms c))"
-    then obtain c' where *: "c2 = c' ;; (While v c) \<and> c' \<in> set (all_subprograms c)" by auto
-    then have "c3 \<in> set (map (\<lambda> x. x ;; (While v c)) (all_subprograms c')) \<or> c3 \<in> set (all_subprograms c')
-      \<or> c3 \<in> set (all_subprograms (While v c))" using 5 by auto
-    then show ?thesis
-    proof (elim disjE)
-      assume "c3 \<in> set (map (\<lambda> x. x ;; (While v c)) (all_subprograms c'))"
-      then have "c3 \<in> set (map (\<lambda> x. x ;; (While v c)) (all_subprograms c))" using * 5 by auto
-      then show ?thesis by auto
-    next
-      assume "c3 \<in> set (all_subprograms c')"
-      then have "c3 \<in> set (all_subprograms c)" using * 5 by auto
-      then show ?thesis by auto
-    next
-      assume "c3 \<in> set (all_subprograms (While v c))"
-      then show ?thesis using 5 by (metis enumerate_subprograms_def set_remdups)
-    qed
-  qed
-qed auto
-
-lemma enumerate_subprograms_complete: "(c1, s1)\<rightarrow>\<^bsup>t\<^esup> (c2, s2)
-  \<Longrightarrow>  c2 \<in> set (enumerate_subprograms c1)"
-proof(induction t arbitrary: c1 s1 c2 s2)
-  case 0
-  then show ?case using c_in_all_subprograms_c by auto
-next
-  case (Suc t)
-  then obtain c1' s1' where "((c1, s1) \<rightarrow> (c1', s1')) \<and> ((c1', s1')\<rightarrow>\<^bsup>t\<^esup> (c2, s2))" by auto
-  then show ?case using enumerate_subprograms_transitive Suc enumerate_subprograms_complete_step 
-    by blast
-qed
-
-lemma SKIP_in_enumerate_subprograms[simp]: "SKIP \<in> set (enumerate_subprograms c)" 
-  by (induction c rule: all_subprograms.induct) auto
-
-lemma enumerate_subprogams_enumerate_variables: "c' \<in> set (enumerate_subprograms c) 
-  \<Longrightarrow> set (all_variables c') \<subseteq> set (enumerate_variables c)" 
-  by (auto simp: enumerate_variables_def)
-
-lemma enumerate_subprograms_max_constant: "c' \<in> set (enumerate_subprograms c)
-  \<Longrightarrow> max_constant c' \<le> max_constant c"
-  by (induction c arbitrary: c' rule: all_subprograms.induct)
-       (fastforce  split: if_splits)+
-
-fun index_of :: "'a list \<Rightarrow> 'a \<Rightarrow> nat" where
-"index_of [] c = 0" |
-"index_of (d # cs) c = (if d = c then 0 else Suc (index_of cs c))"
-
-lemma index_of_element_in_list:
-  "x \<in> set l \<Longrightarrow> index_of l x < length l"
-  by (induction l) auto
-
-lemma index_of_identity[simp]:
-  "x \<in> set l \<Longrightarrow> (l ! (index_of l x) = x)"
-  by (induction l) auto
-
-fun index_of2 :: "('a \<times> 'b) list \<Rightarrow> 'a \<Rightarrow> nat" where
-"index_of2 [] c = 0" |
-"index_of2 ((d,_) # cs) c = (if d = c then 0 else Suc (index_of2 cs c))" 
-
-lemma index_of2_in_list: "x \<in> set (map fst l) \<Longrightarrow> (\<forall>y. (x, y) \<in> set l \<longrightarrow> P y) 
-  \<Longrightarrow> P (snd (l ! (index_of2 l x)))"
-  apply (induction l) 
-   apply auto
-  by force
-
-lemma index_of2_distinct: "(x, y) \<in> set l \<Longrightarrow> distinct (map fst l) 
-  \<Longrightarrow> l ! (index_of2 l x) = (x, y)"
-  apply(induction l)
-   apply(auto)
-  by force
-
-definition pc_to_com :: "com list \<Rightarrow> (variable \<times> domain_element) list \<Rightarrow> com" where
-"pc_to_com cs as = cs ! (case snd (as ! (index_of2 as PC)) of Num x \<Rightarrow> x)"
-
-lemma index_of2_index_of2[simp]: "x \<in> set (map fst l) 
-  \<Longrightarrow> l[index_of2 l x := (x, y)] ! index_of2 (l[index_of2 l x := (x, y)]) x = (x, y)"
-proof (induction l)
-  case (Cons a l)
-  then have "fst a = x \<or> fst a \<noteq> x" by simp
-  then show ?case
-  proof (elim disjE)
-    assume "fst a = x"
-    then show ?thesis using Cons 
-      by (metis eq_fst_iff index_of2.simps length_map length_pos_if_in_set list_update_code nth_list_update)
-  next
-    assume "fst a \<noteq> x"
-    then show ?thesis using Cons 
-      by (metis index_of2.simps list.simps(9) list_update_code nth_Cons_Suc prod.collapse set_ConsD)
-  qed
-qed auto
-
-lemma pc_to_com_of_subprogram: "c1 \<in> set cs \<Longrightarrow> PC \<in> set (map fst as) 
-  \<Longrightarrow> pc_to_com cs
-    (as [index_of2 as PC := (PC, Num (index_of cs c1))]) = c1"
-  by (induction cs) (auto simp: pc_to_com_def)
-
-
-fun com_to_operators :: "com list \<Rightarrow> com \<Rightarrow> domain_element list \<Rightarrow> operator list" where
-"com_to_operators cs (SKIP) d = []" |
-"com_to_operators cs (v ::= aexp) d = (let i = index_of cs (v ::= aexp) ; j = index_of cs SKIP in
+fun com_to_operators :: "com \<Rightarrow> domain_element list \<Rightarrow> operator list" where
+"com_to_operators (SKIP) d = []" |
+"com_to_operators (v ::= aexp) d = 
   (case aexp of
     A a \<Rightarrow> (case a of
-      N val \<Rightarrow> [\<lparr> precondition_of = [(PC, Num i)], 
-                  effect_of = [(PC, Num j), (VN v, (if (Num val) \<in> set d then Num val else \<omega>))]\<rparr>] |
-      V var \<Rightarrow> map (\<lambda> x. \<lparr> precondition_of = [(PC, Num i), (VN var, x)], 
-                           effect_of = [(PC, Num j), (VN v, x)]\<rparr>) d) |
-    Plus a b \<Rightarrow> map (\<lambda> x.  \<lparr> precondition_of = [(PC, Num i), (VN a, x)], 
-                             effect_of = [(PC, Num j), (VN v, (case x of 
-      Num y \<Rightarrow> if Num (y + b) \<in> set d then Num (y + b) else \<omega> | 
-      \<omega> \<Rightarrow> \<omega>))]\<rparr>) d | 
-    Sub a b \<Rightarrow> map (\<lambda> x.  \<lparr> precondition_of = [(PC, Num i), (VN a, x)], 
-                            effect_of = [(PC, Num j), (VN v, (case x of 
-      Num y \<Rightarrow> if Num (y - b) \<in> set d then Num (y - b) else \<omega> | 
-      \<omega> \<Rightarrow> \<omega>))]\<rparr>) d))" |
-"com_to_operators cs (c1;; c2) d = (let i = index_of cs (c1 ;; c2) in 
-  (if c1 = SKIP then (let j = index_of cs c2 in [\<lparr> precondition_of = [(PC, Num i)],
-                                                   effect_of = [(PC, Num j)]\<rparr>])
-   else (let ops = com_to_operators cs c1 d in map (\<lambda> op. 
-    (let j = index_of cs ((pc_to_com cs (effect_of op) ;; c2)) in 
+      N val \<Rightarrow> [\<lparr> precondition_of = [(PC, PCV (v ::= aexp))], 
+                  effect_of = [(PC, PCV SKIP), (VN v, (if (EV (Num val)) \<in> set d then EV (Num val) else EV \<omega>))]\<rparr>] |
+      V var \<Rightarrow> map (\<lambda> x. \<lparr> precondition_of = [(PC, PCV (v ::= aexp)), (VN var, x)], 
+                           effect_of = [(PC, PCV SKIP), (VN v, x)]\<rparr>) d) |
+    Plus a b \<Rightarrow> map (\<lambda> x.  \<lparr> precondition_of = [(PC, PCV (v ::= aexp)), (VN a, x)], 
+                             effect_of = [(PC, PCV SKIP), (VN v, (case x of 
+      EV (Num y) \<Rightarrow> EV (if EV (Num (y + b)) \<in> set d then Num (y + b) else \<omega>) | 
+      _ \<Rightarrow> EV \<omega>))]\<rparr>) d | 
+    Sub a b \<Rightarrow> map (\<lambda> x.  \<lparr> precondition_of = [(PC, PCV (v ::= aexp)), (VN a, x)], 
+                            effect_of = [(PC, PCV SKIP), (VN v, (case x of 
+      EV (Num y) \<Rightarrow> EV (if EV (Num (y - b)) \<in> set d then Num (y - b) else \<omega>) | 
+      _ \<Rightarrow> EV \<omega>))]\<rparr>) d)" |
+"com_to_operators (c1;; c2) d = 
+  (if c1 = SKIP then  [\<lparr> precondition_of = [(PC, PCV (c1 ;; c2))],
+                                                   effect_of = [(PC, PCV c2)]\<rparr>]
+   else (let ops = com_to_operators c1 d in map (\<lambda> op. 
+    (let c1' = pc_to_com (effect_of op) in 
       \<lparr> precondition_of = 
-        list_update (precondition_of op) 
-                    (index_of2 (precondition_of op) PC) (PC, Num i),
+        list_update (precondition_of op) 0 (PC, PCV (c1 ;; c2)),
         effect_of = 
-        list_update (effect_of op) 
-                    (index_of2 (effect_of op) PC) (PC, Num j)\<rparr>)) ops)))" |
-"com_to_operators cs (IF v\<noteq>0 THEN c1 ELSE c2) d = (let i = index_of cs (IF v\<noteq>0 THEN c1 ELSE c2) ;
-  j = index_of cs c1 ; k = index_of cs c2 in map (\<lambda> x. 
-    \<lparr> precondition_of = [(PC, Num i), (VN v, x)], 
-      effect_of = [(PC, (if x = Num 0 then Num k else Num j))]\<rparr>) d)" |
-"com_to_operators cs (WHILE v\<noteq>0 DO c) d = (let i = index_of cs (WHILE v\<noteq>0 DO c) ;
-  j = index_of cs (c ;; (WHILE v\<noteq>0 DO c)); k = index_of cs SKIP in map (\<lambda> x. 
-    \<lparr> precondition_of = [(PC, Num i), (VN v, x)], 
-      effect_of = [(PC, (if x = Num 0 then Num k else Num j))]\<rparr>) d)"
+        list_update (effect_of op) 0 (PC, PCV (c1' ;; c2))\<rparr>)) ops))" |
+"com_to_operators (IF v\<noteq>0 THEN c1 ELSE c2) d = (let i = PCV (IF v\<noteq>0 THEN c1 ELSE c2)
+   in map (\<lambda> x. 
+    \<lparr> precondition_of = [(PC, i), (VN v, x)], 
+      effect_of = [(PC, PCV (if x = EV (Num 0) then c2 else c1))]\<rparr>) d)" |
+"com_to_operators (WHILE v\<noteq>0 DO c) d = (let i = PCV (WHILE v\<noteq>0 DO c) ;
+  j = PCV (c ;; (WHILE v\<noteq>0 DO c)); k = PCV SKIP in map (\<lambda> x. 
+    \<lparr> precondition_of = [(PC, i), (VN v, x)], 
+      effect_of = [(PC, (if x = EV (Num 0) then k else j))]\<rparr>) d)"
 
-lemma PC_in_update: 
-"(PC, y1) \<in> set l \<Longrightarrow> (\<exists>y2. (PC, y2) \<in> set (list_update l (index_of2 l PC) (PC, y3)))" 
-proof (induction l)
-  case (Cons a l)
-  then show ?case 
-    by (metis index_of2.simps list.set_intros list.set_intros list_update_code list_update_code prod.collapse set_ConsD)
-qed auto
+lemma precondition_nonempty[simp]: "op \<in> set (com_to_operators c d) 
+  \<Longrightarrow> length (precondition_of op) > 0"
+  by (induction c d arbitrary: op rule: com_to_operators.induct)
+    (auto split: aexp.splits if_splits atomExp.splits)
 
-lemma PC_in_effect_precondition: "op \<in> set (com_to_operators cs c d) 
-  \<Longrightarrow> (\<exists>y1 y2. (PC, y1) \<in> set (precondition_of op) \<and> (PC, y2) \<in> set (effect_of op))"
-proof(induction cs c d arbitrary: op rule: com_to_operators.induct)
-  case (2 cs v aexp d)
+lemma effect_nonempty[simp]: "op \<in> set (com_to_operators c d) 
+  \<Longrightarrow> length (effect_of op) > 0"
+  by (induction c d arbitrary: op rule: com_to_operators.induct)
+    (auto split: aexp.splits if_splits atomExp.splits)
+
+lemma PC_in_effect_precondition: "op \<in> set (com_to_operators c d) 
+  \<Longrightarrow> (\<exists>y1 y2. (PC, PCV y1) = (precondition_of op) ! 0 \<and> (PC, PCV y2) = (effect_of op) ! 0)"
+proof(induction c d arbitrary: op rule: com_to_operators.induct)
+  case (2 v aexp d)
   then show ?case by (cases aexp) (auto simp: Let_def split: atomExp.splits)
 next
-  case (3 cs c1 c2 d)
+  case (3 c1 c2 d)
   have "c1 = SKIP \<or> c1 \<noteq> SKIP" by simp
-  then show ?case using 3 PC_in_update by fastforce
+  then show ?case using 3 precondition_nonempty effect_nonempty by (auto split: if_splits)
 qed auto
 
-lemma update_PC_registers_unchanged: 
-    "{x \<in> set l. fst x \<noteq> PC} =  {x \<in> set (list_update l (index_of2 l PC) (PC, y)). fst x \<noteq> PC}"
-proof (induction l)
-  case Nil
-  then show ?case by auto
-next
-  case (Cons a l)
-  have "fst a = PC \<or> fst a \<noteq> PC" by auto
-  then show ?case
-  proof (elim disjE)
-    assume "fst a = PC" 
-    then show ?thesis 
-      by (metis (no_types, lifting) Collect_cong fst_conv index_of2.simps list.set_intros 
-         list_update_code prod.collapse set_ConsD)
-  next
-    assume "fst a \<noteq> PC"
-    then have "index_of2 (a#l) PC \<noteq> 0" by (metis index_of2.simps old.nat.distinct prod.collapse)
-    then show ?thesis using Cons 
-      by (smt Collect_cong index_of2.elims insert_iff list.inject list.set list_update_code mem_Collect_eq)
-  qed
-qed
+lemma fst_of_effect[simp]: "op \<in> set (com_to_operators c d) 
+  \<Longrightarrow> fst (effect_of op ! 0) = PC" 
+  using PC_in_effect_precondition by (metis fst_conv)
+
+lemma fst_of_precondition[simp]: "op \<in> set (com_to_operators c d) 
+  \<Longrightarrow> fst (precondition_of op ! 0) = PC" 
+  using PC_in_effect_precondition by (metis fst_conv)
 
 lemma com_to_operators_seq_registers:
-  assumes "c1 \<noteq> SKIP" and  "op \<in> set (com_to_operators cs (c1 ;; c2) d)" 
+  assumes "c1 \<noteq> SKIP" and  "op \<in> set (com_to_operators (c1 ;; c2) d)" 
     and "(VN x, y) \<in> set (precondition_of op) \<or> (VN x, y) \<in> set (effect_of op)"
-  shows "\<exists>op'. op' \<in> set (com_to_operators cs c1 d) 
+  shows "\<exists>op'. op' \<in> set (com_to_operators c1 d) 
           \<and> ((VN x, y) \<in> set (precondition_of op') \<or> (VN x, y) \<in> set (effect_of op'))"
 proof -
-  let ?i = "index_of cs (c1 ;; c2)"
-  obtain op' where "op' \<in> set (com_to_operators cs c1 d) 
-    \<and> op = (let j = index_of cs ((pc_to_com cs (effect_of op') ;; c2)) in 
+  obtain op' where "op' \<in> set (com_to_operators c1 d) 
+    \<and> op = (let c1' = pc_to_com (effect_of op') in 
       \<lparr> precondition_of = 
-        list_update (precondition_of op') 
-                    (index_of2 (precondition_of op') PC) (PC, Num ?i),
+        list_update (precondition_of op') 0 (PC, PCV (c1 ;; c2)),
         effect_of = 
-        list_update (effect_of op') 
-                    (index_of2 (effect_of op') PC) (PC, Num j)\<rparr>)" using assms by auto
+        list_update (effect_of op') 0 (PC, PCV (c1' ;; c2))\<rparr>)" using assms by auto
   moreover then have "(VN x, y) \<in> set (precondition_of op') \<or> (VN x, y) \<in> set (effect_of op')" 
-    using assms update_PC_registers_unchanged by fastforce
+    using assms PC_in_effect_precondition precondition_nonempty effect_nonempty 
+    by (metis (no_types, lifting) eq_fst_iff in_set_conv_nth length_list_update nth_list_update 
+        sas_plus_operator.select_convs sas_plus_operator.select_convs variable.simps)
   ultimately show ?thesis by auto
 qed
 
 lemma com_to_operators_registers_in_d: 
-  "op \<in> set (com_to_operators cs c d) 
-  \<Longrightarrow> ((VN x, y) \<in> set (precondition_of op) \<or> (VN x, y) \<in> set (effect_of op)) \<Longrightarrow> \<omega> \<in> set d 
+  "op \<in> set (com_to_operators c d) 
+  \<Longrightarrow> ((VN x, y) \<in> set (precondition_of op) \<or> (VN x, y) \<in> set (effect_of op)) \<Longrightarrow> EV \<omega> \<in> set d 
   \<Longrightarrow> y \<in> set d"
-proof (induction cs c d arbitrary: op rule: com_to_operators.induct)
-  case (2 cs v aexp d)
-  then show ?case by (auto simp: Let_def split: aexp.splits atomExp.splits if_splits domain_element.splits)
-next
-  case (3 cs c1 c2 d)
+proof (induction c d arbitrary: op rule: com_to_operators.induct)
+  case (3 c1 c2 d)
   have "c1 = SKIP \<or> c1 \<noteq> SKIP" by simp
   then show ?case
   proof (elim disjE)
     assume "c1 \<noteq> SKIP"
-    then show ?thesis using 3 com_to_operators_seq_registers by metis
+    then show ?thesis using 3 com_to_operators_seq_registers by blast
   next
     assume "c1 = SKIP" 
     then show ?thesis using 3 by auto
   qed
-qed (auto simp: Let_def split: aexp.splits atomExp.splits if_splits)
+qed (auto simp: Let_def split: aexp.splits atomExp.splits if_splits domain_element.splits EVal.splits)
 
-lemma update_index_of2_preserve_set:
-  "set (map fst l) = set (map fst (list_update l (index_of2 l x) (x, y)))"
-proof (induction l)
-  case (Cons a l)
-  then show ?case
-    by (metis eq_fst_iff index_of2.simps list.set list.simps list_update_code list_update_code surjective_pairing)
-qed auto
-
-lemma update_index_of2_preserve_distinct: "distinct (map fst l)
-  \<Longrightarrow> distinct (map fst (list_update l (index_of2 l x) (x, y)))"
-proof (induction l)
-  case Nil
-  then show ?case by auto
-next
-  case (Cons a l)
-  let ?l' = "list_update l (index_of2 l x) (x, y)"
-  have "fst a = x \<or> fst a \<noteq> x" by auto
-  then show ?case
-  proof(elim disjE)
-    assume "fst a = x"
-    then show ?thesis using Cons 
-      by (metis (no_types, lifting) eq_fst_iff index_of2.simps list_update_code map_update)
-  next
-    assume "fst a \<noteq> x"
-    then show ?thesis using Cons update_index_of2_preserve_set 
-      by (metis card_distinct distinct_card length_list_update length_map)
-  qed
-qed
+lemma update_preserve_distinct: "distinct (map fst l) \<Longrightarrow> fst (l ! 0) = x 
+  \<Longrightarrow> distinct (map fst (l[0 := (x, y)]))"
+  by (induction l) auto
 
 lemma com_to_operators_variables_distinct: 
-  "op \<in> set (com_to_operators cs c d) \<Longrightarrow> (l = precondition_of op \<or> l = effect_of op)
+  "op \<in> set (com_to_operators c d) \<Longrightarrow> (l = precondition_of op \<or> l = effect_of op)
   \<Longrightarrow> distinct (map fst l)"
-proof(induction cs c d arbitrary: op l rule: com_to_operators.induct)
-  case (3 cs c1 c2 d)
-  have "c1 = SKIP \<or> c1 \<noteq> SKIP" by simp
-  then show ?case using 3 update_index_of2_preserve_distinct by fastforce
-qed (auto simp: Let_def split: aexp.splits atomExp.splits if_splits)
+by (induction c d arbitrary: op l rule: com_to_operators.induct)
+ (auto simp: Let_def update_preserve_distinct split: aexp.splits atomExp.splits if_splits)
+
+lemma PC_of_precondition[simp]: "op \<in> set (com_to_operators c d) 
+  \<Longrightarrow> (PC, y) \<in> set (precondition_of op) \<longleftrightarrow> y = PCV c"
+  using com_to_operators_variables_distinct PC_in_effect_precondition
+  apply(cases c)
+      apply(auto simp: pc_to_com_def split: aexp.splits atomExp.splits if_splits)
+  by(metis eq_key_imp_eq_value fst_of_precondition precondition_nonempty 
+      set_update_memI update_preserve_distinct)+
+
+lemma [simp]: "op \<in> set (com_to_operators c d) 
+  \<Longrightarrow> (map_of (precondition_of op)) PC = Some (PCV c)"
+  using PC_of_precondition com_to_operators_variables_distinct by auto
+
+lemma [simp]: "op \<in> set (com_to_operators c d) 
+  \<Longrightarrow> pc_to_com (precondition_of op) = c"
+  using PC_of_precondition  
+  by (metis PC_in_effect_precondition domain_element.simps nth_mem old.prod.case pc_to_com_def 
+      precondition_nonempty)
+
+lemma [simp]: "op \<in> set (com_to_operators c d) 
+  \<Longrightarrow> (PC, y) \<in> set (effect_of op) \<longleftrightarrow> y = PCV (pc_to_com (effect_of op))"
+  using com_to_operators_variables_distinct PC_in_effect_precondition 
+  by (auto simp: pc_to_com_def)
+   (metis domain_element.simps effect_nonempty eq_key_imp_eq_value nth_mem old.prod.case)+
 
 lemma com_to_operators_PC_is_subprogram: 
-  "cs = enumerate_subprograms c \<Longrightarrow> c1 \<in> set cs \<Longrightarrow> op \<in> set (com_to_operators cs c1 d)
-  \<Longrightarrow> ((PC, y) \<in> set (precondition_of op) \<or> (PC, y) \<in> set (effect_of op))
-  \<Longrightarrow>  (pc_to_com cs (precondition_of op) \<in> set (enumerate_subprograms c1)
-      \<and> pc_to_com cs (effect_of op) \<in> set (enumerate_subprograms c1)
-      \<and> y \<in> set (map (\<lambda> i. Num i) [0..<(length cs)]))"
-proof (induction cs c1 d arbitrary: y op rule: com_to_operators.induct)
-  case (2 cs v aexp d)
-  moreover then have "v ::= aexp \<in> set cs" and "SKIP \<in> set cs" 
-    using SKIP_in_enumerate_subprograms by blast+
-  ultimately show ?case 
-    by (auto simp: Let_def pc_to_com_def index_of_element_in_list split: aexp.splits atomExp.splits)
-next
-  case (3 cs c1 c2 d)
-  then have c1c2_in_cs: "c1 ;; c2 \<in> set (enumerate_subprograms c) 
-    \<and> c1 \<in> set (enumerate_subprograms (c1 ;; c2)) \<and> c2 \<in> set (enumerate_subprograms (c1 ;; c2))" 
-    using c_in_all_subprograms_c by auto
-  then have "c1 \<in> set (enumerate_subprograms c) \<and> c2 \<in> set (enumerate_subprograms c)" 
-    using enumerate_subprograms_transitive by blast
-  then have c1_in_cs: "c1 \<in> set cs" and c2_in_cs: "c2 \<in> set cs" using 3 by auto
-  then have "c1 = SKIP \<or> c1 \<noteq> SKIP" by auto
-  then show ?case
-  proof (elim disjE)
-    assume "c1 = SKIP"
-    then show ?thesis
-      using 3 c2_in_cs c_in_all_subprograms_c c1c2_in_cs 
-      by (auto simp: Let_def pc_to_com_def index_of_element_in_list)
-  next
-    assume a: "c1 \<noteq> SKIP"
-    moreover then obtain op' where op'_def: "op' \<in> set (com_to_operators cs c1 d)
-      \<and> precondition_of op = list_update (precondition_of op') 
-                    (index_of2 (precondition_of op') PC) (PC, Num (index_of cs (c1 ;; c2)))
-      \<and> effect_of op = list_update (effect_of op') 
-                      (index_of2 (effect_of op') PC) (PC, Num (index_of cs (pc_to_com cs (effect_of op') ;; c2)))"
-      using 3 a by (auto simp: Let_def)
-    moreover then obtain c3 where c3_def: "c3 = pc_to_com cs (effect_of op')" by auto
-    ultimately have "c3 \<in> set (enumerate_subprograms c1)" using 3 c1_in_cs
-      by (meson PC_in_effect_precondition)
-    then have "c3 ;; c2 \<in> set (enumerate_subprograms (c1 ;; c2))" by auto
-    then have *: "c3 ;; c2 \<in> set cs" and **: "c1 ;; c2 \<in> set cs" using enumerate_subprograms_transitive 
-      using 3 "3.prems"(1) c1c2_in_cs by (meson PC_in_effect_precondition)+
-    have ***: "PC \<in> set (map fst (precondition_of op'))" and ****: "PC \<in> set (map fst (effect_of op'))"
-      using PC_in_effect_precondition 3 op'_def by (metis in_set_zipE zip_map_fst_snd)+
-    have "pc_to_com cs (precondition_of op) = c1 ;; c2" 
-      using op'_def pc_to_com_of_subprogram[OF ** ***] by auto 
-    moreover have "pc_to_com cs (effect_of op) = c3 ;; c2"
-      using op'_def pc_to_com_of_subprogram[OF * ****] using c3_def by auto
-    moreover have "y = Num (index_of cs (c1 ;; c2)) \<or> y = Num (index_of cs (c3 ;; c2))" 
-      using 3 op'_def c3_def com_to_operators_variables_distinct *** ****
-      by (metis Pair_inject index_of2_distinct index_of2_index_of2)
-    ultimately show ?thesis 
-      using c_in_all_subprograms_c \<open>c3;; c2 \<in> set (enumerate_subprograms (c1;; c2))\<close> 3 *
-      by (auto simp: index_of_element_in_list)
-  qed
-next
-  case (4 cs v c1 c2 d)
-  let ?i = "IF v \<noteq>0 THEN c1 ELSE c2"
-  have "?i \<in> set (enumerate_subprograms c) \<and> c1 \<in> set (enumerate_subprograms ?i) \<and> c2 \<in> set (enumerate_subprograms ?i)" 
-    using 4 c_in_all_subprograms_c by auto
-  moreover then have "c1 \<in> set (enumerate_subprograms c) \<and> c2 \<in> set (enumerate_subprograms c)"
-    using enumerate_subprograms_transitive by blast
-  ultimately have "?i \<in> set cs \<and> c1 \<in> set cs \<and> c2 \<in> set cs" using 4 by auto
-  then show ?case using 4 c_in_all_subprograms_c 
-    by (auto simp: Let_def pc_to_com_def index_of_element_in_list) 
-next
-  case (5 cs v c1 d)
-  let ?w = "WHILE v \<noteq>0 DO c1"
-  have "?w \<in> set (enumerate_subprograms c) \<and> c1 ;; ?w \<in> set (enumerate_subprograms ?w)" 
-    using 5 c_in_all_subprograms_c by auto
-  moreover then have "c1 ;; ?w \<in> set (enumerate_subprograms c)"
-    using enumerate_subprograms_transitive by blast
-  ultimately have "?w \<in> set cs \<and> c1 ;; ?w \<in> set cs \<and> SKIP \<in> set cs" 
-    using 5 SKIP_in_enumerate_subprograms by auto
-  then show ?case using 5 c_in_all_subprograms_c 
-    by (auto simp: Let_def pc_to_com_def index_of_element_in_list) 
-qed auto
+  "op \<in> set (com_to_operators c d)
+  \<Longrightarrow>  (pc_to_com (precondition_of op) \<in> set (enumerate_subprograms c)
+      \<and> pc_to_com (effect_of op) \<in> set (enumerate_subprograms c))"
+  apply (induction c d arbitrary: op rule: com_to_operators.induct)
+  using c_in_all_subprograms_c precondition_nonempty effect_nonempty
+      by (auto simp: Let_def pc_to_com_def split: if_splits aexp.splits atomExp.splits)
 
-lemma com_to_operators_variables_in_enumerate_variables: "cs = (enumerate_subprograms c) ==> c1 \<in> set cs
-  \<Longrightarrow> op \<in> set (com_to_operators cs c1 d)
+lemma com_to_operators_variables_in_enumerate_variables: "op \<in> set (com_to_operators c d)
   \<Longrightarrow> ((VN x, y) \<in> set (precondition_of op) \<or> (VN x, y) \<in> set (effect_of op))
   \<Longrightarrow> x \<in> set (enumerate_variables c)"
-proof (induction cs c1 d arbitrary: op rule: com_to_operators.induct)
-  case (1 cs d)
-  then show ?case by auto
-next
-  case (2 cs v aexp d)
-  then have "set (all_variables (v ::= aexp)) \<subseteq> set (enumerate_variables c)" 
-    using enumerate_subprogams_enumerate_variables by blast 
-  then show ?case using 2 by (auto simp: Let_def split: aexp.splits atomExp.splits if_splits) 
-next
-  case (3 cs c1 c2 d)
+proof (induction c d arbitrary: op rule: com_to_operators.induct)
+  case (3 c1 c2 d)
   have "c1 = SKIP \<or> c1 \<noteq> SKIP" by auto
   then show ?case
   proof (elim disjE)
@@ -437,53 +189,65 @@ next
     then show ?thesis using 3 by auto
   next
     assume "c1 \<noteq> SKIP"
-    then obtain op' where "op' \<in> set (com_to_operators cs c1 d) 
+    moreover then obtain op' where "op' \<in> set (com_to_operators c1 d) 
           \<and> ((VN x, y) \<in> set (precondition_of op') \<or> (VN x, y) \<in> set (effect_of op'))"
       using 3 com_to_operators_seq_registers by presburger
-    moreover have "c1 ;; c2 \<in> set (enumerate_subprograms c) \<and> c1 \<in> set (enumerate_subprograms (c1 ;; c2))" 
-      using 3 c_in_all_subprograms_c by simp
-    moreover then have "c1 \<in> set (enumerate_subprograms c)" 
-      using 3 enumerate_subprograms_transitive by blast
-    ultimately show ?thesis using 3 \<open>c1 \<noteq> SKIP\<close> by blast
+    moreover have "c1 \<in> set (enumerate_subprograms (c1 ;; c2))" using c_in_all_subprograms_c by auto
+    moreover then have "set (enumerate_variables c1) \<subseteq> set (enumerate_variables (c1 ;; c2))"
+      using enumerate_subprograms_enumerate_variables
+      by simp
+    ultimately show ?thesis using 3 by auto
   qed
-next
-  case (4 cs v c1 c2 d)
-  then have "set (all_variables (IF v \<noteq>0 THEN c1 ELSE c2)) \<subseteq> set (enumerate_variables c)" 
-    using enumerate_subprogams_enumerate_variables by blast 
-  then show ?case using 4 by (auto simp: Let_def split: aexp.splits atomExp.splits if_splits)
-next
-  case (5 cs v c' d)
-  then have "set (all_variables (WHILE v \<noteq>0 DO c')) \<subseteq> set (enumerate_variables c)" 
-    using enumerate_subprogams_enumerate_variables by blast
-  then show ?case using 5 by (auto simp: Let_def split: aexp.splits atomExp.splits if_splits)
-qed
+qed (auto simp: Let_def  split: aexp.splits atomExp.splits if_splits)
+
+lemma [simp]: 
+  assumes "op \<in> set (com_to_operators c1 d)"
+    "(a, b) \<in> set (precondition_of op)"
+    "c1 \<in> set (enumerate_subprograms c)"
+    "a \<notin> VN ` set (enumerate_variables c)" 
+  shows "a = PC"
+proof (cases a)
+  case (VN v)
+  have "set (enumerate_variables c1) \<subseteq> set (enumerate_variables c)" 
+    using assms enumerate_subprograms_enumerate_variables by auto
+  then show ?thesis using VN com_to_operators_variables_in_enumerate_variables assms by blast
+qed auto
+
+lemma [simp]: 
+  assumes "op \<in> set (com_to_operators c1 d)"
+    "(a, b) \<in> set (effect_of op)"
+    "c1 \<in> set (enumerate_subprograms c)"
+    "a \<notin> VN ` set (enumerate_variables c)" 
+  shows "a = PC"
+proof (cases a)
+  case (VN v)
+  have "set (enumerate_variables c1) \<subseteq> set (enumerate_variables c)" 
+    using assms enumerate_subprograms_enumerate_variables by auto
+  then show ?thesis using VN com_to_operators_variables_in_enumerate_variables assms by blast
+qed auto
 
 definition coms_to_operators :: "com list \<Rightarrow> domain_element list \<Rightarrow> operator list" where
-"coms_to_operators cs d = concat (map (\<lambda> c. com_to_operators cs c d) cs)"
+"coms_to_operators cs d = concat (map (\<lambda> c. com_to_operators c d) cs)"
 
 definition sas_state_by_pc_and_vars :: 
   "com list \<Rightarrow> com  \<Rightarrow> (vname \<rightharpoonup> nat) \<Rightarrow> domain_element list \<Rightarrow> sas_state" where
 "sas_state_by_pc_and_vars cs c vs d =  (\<lambda> v. (case v of 
-  VN vn \<Rightarrow> (case vs vn of Some x \<Rightarrow> (if Num x \<in> set d then Some (Num x) else Some \<omega>) |
+  VN vn \<Rightarrow> (case vs vn of Some x \<Rightarrow> (if EV (Num x) \<in> set d then Some (EV (Num x)) else Some (EV \<omega>)) |
                           None \<Rightarrow> None) |
-  PC \<Rightarrow> Some (Num (index_of cs c))))"
+  PC \<Rightarrow> Some (PCV c)))"
 
 lemma sas_state_by_pc_and_vars_variables_in_d: 
   "x \<noteq> PC \<Longrightarrow> (sas_state_by_pc_and_vars cs c vs d) x = Some y 
-  \<Longrightarrow> (y = \<omega> \<or> y \<in> set d)"
+  \<Longrightarrow> (y = EV \<omega> \<or> y \<in> set d)"
   by (auto simp: sas_state_by_pc_and_vars_def split: variable.splits option.splits if_splits)
-
-lemma sas_state_by_pc_and_vars_PC_in_d:
-  "c \<in> set cs \<Longrightarrow> (sas_state_by_pc_and_vars cs c vs d) PC = Some y
-  \<Longrightarrow> y \<in> set (map (\<lambda> i. Num i) [0..<(length cs)])"
-  by (auto simp: sas_state_by_pc_and_vars_def index_of_element_in_list split: variable.splits option.splits if_splits)
 
 definition imp_minus_minus_to_sas_plus :: "com \<Rightarrow> (vname \<rightharpoonup> nat) \<Rightarrow> nat \<Rightarrow> problem" where
 "imp_minus_minus_to_sas_plus c vs t = (let cs = enumerate_subprograms c ; 
   d = domain c t ; 
-  initial_vs = (\<lambda>x. (if x \<in> set (enumerate_variables c) then Some (case vs x of Some y \<Rightarrow> y | None \<Rightarrow> 0)
+  initial_vs = (\<lambda>x. (if x \<in> set (enumerate_variables c) 
+      then Some (case vs x of Some y \<Rightarrow> y | None \<Rightarrow> 0)
     else None)) ;
-  pc_d = map (\<lambda> i. Num i) [0..<(length cs)] in
+  pc_d = map (\<lambda> i. PCV i) (enumerate_subprograms c) in
     \<lparr> variables_of = PC # (map (\<lambda> v. VN v) (enumerate_variables c)),
       operators_of = coms_to_operators cs d, 
       initial_of = sas_state_by_pc_and_vars cs c initial_vs d,
@@ -495,14 +259,10 @@ lemma range_defined:
   shows "(\<exists>y. range_of (imp_minus_minus_to_sas_plus c vs t) v = Some y)"
 proof(cases v)
   case (VN x)
-  then have *: "(VN x, domain c t) \<in> set (map (\<lambda> v. (VN v, domain c t)) (enumerate_variables c))" 
+  then have "(VN x, domain c t) \<in> set (map (\<lambda> v. (VN v, domain c t)) (enumerate_variables c))" 
     using assms by (auto simp: Let_def imp_minus_minus_to_sas_plus_def)    
-  then show ?thesis using VN by (simp add: Let_def imp_minus_minus_to_sas_plus_def) 
-       (smt Pair_inject * ex_map_conv map_of_SomeD weak_map_of_SomeI)
-next
-  case PC
-  then show ?thesis by (auto simp: imp_minus_minus_to_sas_plus_def Let_def)
-qed
+  then show ?thesis using VN by (auto simp: Let_def imp_minus_minus_to_sas_plus_def weak_map_of_SomeI) 
+qed (auto simp: imp_minus_minus_to_sas_plus_def Let_def)
 
 lemma range_non_empty: 
   assumes "v \<in> set (variables_of (imp_minus_minus_to_sas_plus c vs t))" 
@@ -514,24 +274,16 @@ proof (cases v)
   then have "range_of (imp_minus_minus_to_sas_plus c vs t) v = Some (domain c t)" 
     using VN by (simp add: Let_def imp_minus_minus_to_sas_plus_def) 
        (smt Pair_inject * ex_map_conv map_of_SomeD weak_map_of_SomeI)
-  then have "\<omega> \<in> range_of' (imp_minus_minus_to_sas_plus c vs t) v" 
-    by (auto simp: domain_def range_of'_def)
-  then show ?thesis by auto
+  then show ?thesis using assms VN by (simp add: range_of'_def)
+     (meson ListMem_iff omega_in_domain)
 next
   case PC
-  let ?pc_d = "(map (\<lambda> i. Num i) [0..<(length (enumerate_subprograms c))])"
-  have "range_of (imp_minus_minus_to_sas_plus c vs t) v 
-    = Some ?pc_d"
-    using assms PC by (auto simp: Let_def imp_minus_minus_to_sas_plus_def)
-  then have "range_of (imp_minus_minus_to_sas_plus c vs t) v = Some ?pc_d" using PC by simp
-  moreover have "Num 0 \<in> set ?pc_d" using SKIP_in_enumerate_subprograms 
-    by (metis (no_types, lifting) add.left_neutral in_set_conv_nth length_map length_pos_if_in_set map_nth nth_map nth_upt)
-  ultimately have "Num 0 \<in> range_of' (imp_minus_minus_to_sas_plus c vs t) v"
-    by (auto simp: domain_def range_of'_def)
-  then show ?thesis by auto
+  then show ?thesis using SKIP_in_enumerate_subprograms
+    by (auto simp:  range_of'_def Let_def imp_minus_minus_to_sas_plus_def) 
+      (metis empty_iff empty_set) 
 qed
 
-lemma map_of_variables: "x \<in> set l \<Longrightarrow> (map_of (map (\<lambda>v. (VN v, d)) l) (VN x)) = Some d"
+lemma [simp]: "x \<in> set l \<Longrightarrow> (map_of (map (\<lambda>v. (VN v, d)) l) (VN x)) = Some d"
   by (induction l) auto
 
 lemma distinct_list_all: 
@@ -548,56 +300,36 @@ proof -
   then show ?thesis
     by (metis (no_types, lifting) case_prodI2 list.pred_set)
 qed 
-  
+
+lemma [simp]: "PCV x \<in> PCV ` y \<longleftrightarrow> x \<in> y" by auto
 
 lemma operators_valid: 
   assumes "cs = enumerate_subprograms c" and "c1 \<in> set cs" and "d = domain c t"
-         and  "op \<in> set (com_to_operators cs c1 d)"
+         and  "op \<in> set (com_to_operators c1 d)"
   shows "is_valid_operator_sas_plus (imp_minus_minus_to_sas_plus c vs t) op" 
 proof -                   
   let ?\<Psi> = "imp_minus_minus_to_sas_plus c vs t"
   let ?pre = "precondition_of op" and ?eff = "effect_of op" and ?vs = "variables_of ?\<Psi>" 
-      and ?D = "range_of ?\<Psi>" and ?pc_d = "(map (\<lambda> i. Num i) [0..<(length (enumerate_subprograms c))])"
+      and ?D = "range_of ?\<Psi>" and ?pc_d = "map (\<lambda> i. PCV i) (enumerate_subprograms c)"
 
-  have *: "((VN x, a) \<in> set ?pre \<or> (VN x, a) \<in> set ?eff) \<Longrightarrow> x \<in> set (enumerate_variables c)" for x a 
-    using com_to_operators_variables_in_enumerate_variables[OF assms(1) assms(2) assms(4)] by auto
-  then have "((VN x, a) \<in> set ?pre \<or> (VN x, a) \<in> set ?eff) \<Longrightarrow> ListMem (VN x) ?vs" for x a 
-    by (auto simp: imp_minus_minus_to_sas_plus_def Let_def ListMem_iff)
-  moreover have "ListMem PC ?vs" by (auto simp: imp_minus_minus_to_sas_plus_def Let_def ListMem_iff)
-  ultimately have "((v, a) \<in> set ?pre \<or> (v, a) \<in> set ?eff) \<Longrightarrow> ListMem v ?vs" for v a by (cases v) auto
-  then have pre_in_range: "list_all (\<lambda>(v, a). ListMem v ?vs) ?pre" 
-    and eff_in_range: "list_all (\<lambda>(v, a). ListMem v ?vs) ?eff"  
-    by (metis (mono_tags, lifting) case_prodI2 list.pred_set)+
+  have *: "list_all (\<lambda>(v, a). ListMem v ?vs) ?pre \<and> list_all (\<lambda>(v, a). ListMem v ?vs) ?eff"
+    using assms by(auto simp: imp_minus_minus_to_sas_plus_def Let_def ListMem_iff list_all_def)
 
-  have "x \<in> set (enumerate_variables c) \<Longrightarrow> ?D (VN x) = Some d" for x
-    using assms(3) map_of_variables by (simp add: imp_minus_minus_to_sas_plus_def Let_def) fast
-  then have "((VN x, a) \<in> set ?pre \<or> (VN x, a) \<in> set ?eff) \<Longrightarrow> ?D (VN x) = Some d" for x a 
-    using * by (auto simp: imp_minus_minus_to_sas_plus_def Let_def)
-  then have "((VN x, a) \<in> set ?pre \<or> (VN x, a) \<in> set ?eff) \<Longrightarrow> ?D (VN x) = Some d \<and> a \<in> set d" for x a
-    by (metis assms(3) assms(4) com_to_operators_registers_in_d domain_def in_set_conv_decomp)
-  moreover have "((PC, a) \<in> set ?pre \<or> (PC, a) \<in> set ?eff) \<Longrightarrow> ?D PC = Some ?pc_d \<and> a \<in> set ?pc_d" for a
-    using com_to_operators_PC_is_subprogram assms
-    by (metis (no_types, lifting) fun_upd_apply imp_minus_minus_to_sas_plus_def sas_plus_problem.select_convs)
-  ultimately have "((v, a) \<in> set ?pre \<or> (v, a) \<in> set ?eff) \<Longrightarrow> (?D v \<noteq> None \<and> a \<in> set (the (?D v)))" for v a
-    by (cases v) auto
+  have "((VN x, a) \<in> set ?pre \<or> (VN x, a) \<in> set ?eff) \<Longrightarrow> ?D (VN x) = Some d \<and> a \<in> set d" for x a
+    using assms com_to_operators_registers_in_d com_to_operators_variables_in_enumerate_variables
+        enumerate_subprograms_enumerate_variables 
+    by (fastforce simp: imp_minus_minus_to_sas_plus_def Let_def)    
   then have "((v, a) \<in> set ?pre \<or> (v, a) \<in> set ?eff) \<Longrightarrow> (?D v \<noteq> None \<and> ListMem a (the (?D v)))" for v a
-    by (simp add: ListMem_iff)
+    using com_to_operators_PC_is_subprogram assms enumerate_subprograms_transitive
+    by (cases v) 
+      (auto simp: imp_minus_minus_to_sas_plus_def Let_def ListMem_iff Ball_set_list_all)
   then have "list_all (\<lambda>(v, a). (?D v \<noteq> None) \<and> ListMem a (the (?D v))) ?pre" 
     and "list_all (\<lambda>(v, a). (?D v \<noteq> None) \<and> ListMem a (the (?D v))) ?eff" 
     using Ball_set_list_all by blast+
 
   then show ?thesis 
-    using com_to_operators_variables_distinct assms distinct_list_all pre_in_range eff_in_range 
-    apply (auto simp: is_valid_operator_sas_plus_def Let_def) 
-    by blast+ 
-qed
-
-lemma SKIP_in_pcs[simp]:  "ListMem (Num (index_of (enumerate_subprograms c) SKIP))
-     (map Num [0..<length (enumerate_subprograms c)])"
-proof -
-  have "index_of (enumerate_subprograms c) SKIP < length (enumerate_subprograms c)"
-    using SKIP_in_enumerate_subprograms index_of_element_in_list by fastforce
-  then show ?thesis by (simp add: ListMem_iff)
+    using com_to_operators_variables_distinct assms distinct_list_all *
+    by (fastforce simp: is_valid_operator_sas_plus_def Let_def) 
 qed
 
 lemma imp_minus_minus_to_sas_plus_valid: 
@@ -609,48 +341,23 @@ proof -
       and ?I = "initial_of ?\<Psi>"
       and ?G = "goal_of ?\<Psi>"
       and ?D = "range_of ?\<Psi>"
-  have "x \<in> set ?ops \<Longrightarrow> is_valid_operator_sas_plus ?\<Psi> x" for x 
-  proof -
-    assume "x \<in> set ?ops"
-    then have "\<exists>c1 \<in> set (enumerate_subprograms c). 
-      x \<in> set (com_to_operators (enumerate_subprograms c) c1 (domain c t))"
-      by (auto simp: imp_minus_minus_to_sas_plus_def Let_def coms_to_operators_def)
-    then show ?thesis using operators_valid by auto
-  qed
+  have "x \<in> set ?ops \<Longrightarrow> is_valid_operator_sas_plus ?\<Psi> x" for x using operators_valid 
+    by (auto simp: imp_minus_minus_to_sas_plus_def Let_def coms_to_operators_def)
   moreover have "\<forall>v. ?I v \<noteq> None \<longleftrightarrow> ListMem v ?vs"
-  proof
-    fix v
-    show "?I v \<noteq> None \<longleftrightarrow> ListMem v ?vs" 
-      by (cases v) (auto simp: imp_minus_minus_to_sas_plus_def Let_def sas_state_by_pc_and_vars_def ListMem.elem ListMem_iff)
-  qed
+    by (auto simp: imp_minus_minus_to_sas_plus_def Let_def sas_state_by_pc_and_vars_def 
+          ListMem.elem ListMem_iff split: variable.splits)
   moreover have "?I v \<noteq> None \<Longrightarrow> ListMem (the (?I v)) (the (?D v))" for v
-  proof -
-    assume assm: "?I v \<noteq> None" 
-    then show ?thesis
-    proof(cases v)
-      case (VN x1)
-      then have "x1 \<in> set (enumerate_variables c)" 
-        using VN assm by (auto simp: imp_minus_minus_to_sas_plus_def Let_def sas_state_by_pc_and_vars_def split: option.splits if_splits)
-      then have "the (?D v) = domain c t" 
-        using VN by (auto simp: imp_minus_minus_to_sas_plus_def Let_def map_of_variables)
-      then show ?thesis 
-        using VN assm 
-        apply (auto simp: imp_minus_minus_to_sas_plus_def Let_def sas_state_by_pc_and_vars_def elem ListMem_iff split: option.splits)
-        by (meson ListMem_iff omega_in_domain)+
-    next
-      case PC
-      have "c \<in> set (enumerate_subprograms c)" using c_in_all_subprograms_c by auto
-      then show ?thesis using PC 
-        by (auto simp: imp_minus_minus_to_sas_plus_def Let_def sas_state_by_pc_and_vars_def index_of_element_in_list ListMem_iff)
-    qed
-  qed
+    using c_in_all_subprograms_c
+    by (auto simp: imp_minus_minus_to_sas_plus_def Let_def sas_state_by_pc_and_vars_def 
+        ListMem_iff split: variable.splits)
   moreover have "\<forall>v. ?G v \<noteq> None \<longrightarrow> ListMem v ?vs"
-    by (auto simp: imp_minus_minus_to_sas_plus_def Let_def sas_state_by_pc_and_vars_def ListMem.elem split: variable.splits)
+    by (auto simp: imp_minus_minus_to_sas_plus_def Let_def sas_state_by_pc_and_vars_def ListMem.elem 
+        split: variable.splits)
   moreover have "\<forall>v. ?G v \<noteq> None \<longrightarrow> ListMem (the (?G v)) (the (?D v))"
-    using SKIP_in_pcs by (auto simp: imp_minus_minus_to_sas_plus_def Let_def sas_state_by_pc_and_vars_def ListMem.elem split: variable.splits)
-
-  ultimately show ?thesis 
-    by (auto simp: is_valid_problem_sas_plus_def Let_def range_defined list_all_def sas_state_by_pc_and_vars_variables_in_d sas_state_by_pc_and_vars_PC_in_d)
+    using SKIP_in_enumerate_subprograms by (auto simp: imp_minus_minus_to_sas_plus_def Let_def 
+        sas_state_by_pc_and_vars_def ListMem_iff split: variable.splits)
+  ultimately show ?thesis
+    by (auto simp: is_valid_problem_sas_plus_def range_defined list_all_def)
 qed
 
 end
